finish imp.v until ceval_deterministic

ass3/Imp.v
@@ -1620,8 +1620,8 @@ Proof.
       [loopdef] terminates.  Most of the cases are immediately
       contradictory (and so can be solved in one step with
       [discriminate]). *)
-
-  (* FILL IN HERE *) Admitted.
+induction contra; inversion Heqloopdef; subst; try discriminate;
+          apply IHcontra2; reflexivity. Qed.
 (** [] *)
 
 (** **** Exercise: 3 stars, standard (no_whiles_eqv) 
@@ -1648,14 +1648,31 @@ Fixpoint no_whiles (c : com) : bool :=
     while loops.  Then prove its equivalence with [no_whiles]. *)
 
 Inductive no_whilesR: com -> Prop :=
- (* FILL IN HERE *)
+  | nw_skip : no_whilesR <{ skip }>
+  | nw_asgn : forall x exp, no_whilesR <{ x := exp }>
+  | nw_seq : forall cmd1 cmd2 (H1: no_whilesR cmd1) (H2: no_whilesR cmd2), no_whilesR <{ cmd1; cmd2 }>
+  | nw_if : forall bool cmd1 cmd2 (H1: no_whilesR cmd1) (H2: no_whilesR cmd2), no_whilesR <{ if bool then cmd1 else cmd2 end }>
 .
 
 Theorem no_whiles_eqv:
    forall c, no_whiles c = true <-> no_whilesR c.
 Proof.
-  (* FILL IN HERE *) Admitted.
-(** [] *)
+  intros c.
+  split.
+  - intros H. induction c;
+      try constructor;
+      try (inversion H as [H1]);
+      try (apply andb_true_iff in H1);
+      try (destruct H1 as [H1 H2]);
+      try (apply IHc1; apply H1);
+      try (apply IHc2; apply H2).
+  - intros H. induction H; simpl; try reflexivity.
+    + apply andb_true_iff. split.
+      * apply IHno_whilesR1.
+      * apply IHno_whilesR2.
+    + rewrite IHno_whilesR1. simpl. assumption.
+Qed.
+
 
 (** **** Exercise: 4 stars, standard (no_whiles_terminating) 
 
@@ -1664,7 +1681,21 @@ Proof.
 
     Use either [no_whiles] or [no_whilesR], as you prefer. *)
 
-(* FILL IN HERE *)
+Theorem no_whiles_terminating : forall cmd, no_whilesR cmd -> forall st, exists st', st =[ cmd ]=> st'.
+Proof.
+  intros c H.
+  induction H; intros st.
+  - exists st. apply E_Skip.
+  - exists (x !-> (aeval st exp) ; st). constructor. reflexivity.
+  - specialize (IHno_whilesR1 st). destruct IHno_whilesR1 as [st' H1].
+    specialize (IHno_whilesR2 st'). destruct IHno_whilesR2 as [st'' H2].
+    exists st''. apply E_Seq with st'; assumption.
+  - specialize (IHno_whilesR1 st). destruct IHno_whilesR1 as [st' H1].
+    specialize (IHno_whilesR2 st). destruct IHno_whilesR2 as [st'' H2].
+     destruct (beval st bool) eqn:Hbeval.
+     + exists st'. apply E_IfTrue; assumption.
+     + exists st''. apply E_IfFalse; assumption.
+Qed.
 
 (* Do not modify the following line: *)
 Definition manual_grade_for_no_whiles_terminating : option (nat*string) := None.
@@ -1946,31 +1977,70 @@ Reserved Notation "st '=[' c ']=>' st' '/' s"
 Inductive ceval : com -> state -> result -> state -> Prop :=
   | E_Skip : forall st,
       st =[ CSkip ]=> st / SContinue
-  (* FILL IN HERE *)
-
+  | E_Break : forall st,
+      st =[ break ]=> st / SBreak
+  | E_Ass : forall st x a n,
+      aeval st a = n ->
+      st =[ x := a ]=> (x !-> n ; st) / SContinue
+  | E_Seq_Break : forall c1 c2 st st',
+      st =[ c1 ]=> st' / SBreak ->
+      st =[ c1 ; c2 ]=> st' / SBreak
+  | E_Seq_Continue : forall c1 c2 st st' st'' s,
+      st =[ c1 ]=> st' / SContinue ->
+      st' =[ c2 ]=> st'' / s ->
+      st =[ c1 ; c2 ]=> st'' / s
+  | E_IfTrue : forall st st' b c1 c2 s,
+      beval st b = true ->
+      st =[ c1 ]=> st' / s ->
+      st =[ if b then c1 else c2 end ]=> st' / s
+  | E_IfFalse : forall st st' b c1 c2 s,
+      beval st b = false ->
+      st =[ c2 ]=> st' / s ->
+      st =[ if b then c1 else c2 end ]=> st' / s
+   | E_WhileEnd : forall b st c,
+      beval st b = false ->
+      st =[ while b do c end ]=> st / SContinue
+ | E_WhileLoop_Break : forall st st' b c,
+      beval st b = true ->
+      st =[ c ]=> st' / SBreak ->
+      st =[ while b do c end ]=> st' / SContinue
+  | E_WhileLoop_Continue : forall st st' st'' b c,
+      beval st b = true ->
+      st =[ c ]=> st' / SContinue ->
+      st' =[ while b do c end ]=> st'' / SContinue ->
+      st =[ while b do c end ]=> st'' / SContinue
   where "st '=[' c ']=>' st' '/' s" := (ceval c st s st').
+
 
 (** Now prove the following properties of your definition of [ceval]: *)
 
 Theorem break_ignore : forall c st st' s,
      st =[ break; c ]=> st' / s ->
      st = st'.
-Proof.
-  (* FILL IN HERE *) Admitted.
+ Proof.
+  intros.
+    inversion H; 
+    inversion H5. 
+    reflexivity. inversion H2.
+Qed.
 
 Theorem while_continue : forall b c st st' s,
   st =[ while b do c end ]=> st' / s ->
   s = SContinue.
 Proof.
-  (* FILL IN HERE *) Admitted.
+  intros.
+  inversion H;
+  reflexivity.
+Qed.
 
 Theorem while_stops_on_break : forall b c st st',
   beval st b = true ->
   st =[ c ]=> st' / SBreak ->
   st =[ while b do c end ]=> st' / SContinue.
 Proof.
-  (* FILL IN HERE *) Admitted.
-(** [] *)
+  intros b c st st' Hb Hc.
+  eapply E_WhileLoop_Break; assumption.
+Qed.
 
 (** **** Exercise: 3 stars, advanced, optional (while_break_true)  *)
 Theorem while_break_true : forall b c st st',
@@ -1978,8 +2048,80 @@ Theorem while_break_true : forall b c st st',
   beval st' b = true ->
   exists st'', st'' =[ c ]=> st' / SBreak.
 Proof.
-(* FILL IN HERE *) Admitted.
-(** [] *)
+  intros b c st st' Hceval Hb.
+  remember <{ while b do c end }> as loop eqn:Heqloop.
+   induction Hceval;
+   try (inversion Heqloop; subst; simpl in *; congruence).
+    - injection Heqloop as Hb' Hc' ; subst. exists st. assumption.
+    - eauto.
+Qed.
+
+
+Theorem ceval_deterministic2: forall (c:com) st st1 st2 s1 s2,
+     st =[ c ]=> st1 / s1 ->
+     st =[ c ]=> st2 / s2 ->
+     st1 = st2 /\ s1 = s2.
+Proof.
+  intros c st st1 st2 s1 s2 E1 E2.
+  generalize dependent st2.
+  generalize dependent s2.
+  induction E1;
+    intros s2 st2 E2;
+    inversion E2 as [ | | | | | | | | | ];
+    subst;
+    try (split; reflexivity);
+    try (apply IHE1; assumption);
+    try (rewrite H in H0; discriminate).
+  + destruct (IHE1 SContinue st'0). assumption. discriminate.
+  + destruct (IHE1_1 SBreak st2). assumption. discriminate.
+  + destruct (IHE1_1 SContinue st'0). assumption. subst. apply IHE1_2. assumption.
+  + split. apply IHE1 with SBreak. assumption. reflexivity.
+  + destruct (IHE1 SContinue st'0). assumption. discriminate.
+  + destruct (IHE1_1 SBreak st2). assumption. discriminate.
+  + destruct (IHE1_1 SContinue st'0). assumption. subst. apply IHE1_2. assumption.
+Qed.
+Ltac assumption_then_solve :=
+  try assumption; try subst; repeat auto.
+Ltac assumption_then_discriminate :=
+  try assumption; try discriminate.
+
+Ltac destruct_IHHceval1_continue :=
+  match goal with
+  | IHHceval1: forall (s2 : result) (st2 : state),
+               ?st =[ ?c1 ]=> st2 / s2 ->
+               ?st' = st2 /\ SBreak = s2,
+    st'0: state,
+    H : ?st =[ ?c1 ]=> ?st'0 / SContinue
+    |- _ =>
+    destruct (IHHceval1 SContinue st'0) as [H']
+
+   | IHHceval1: forall (s2 : result) (st2 : state),
+               ?st =[ ?c1 ]=> st2 / s2 ->
+               ?st' = st2 /\ SBreak = s2,
+    st'0: state,
+    H : ?st =[ ?c1 ]=> ?st2 / SBreak
+    |- _ =>
+    destruct (IHHceval1 SBreak st2) as [H']
+
+  | IHHceval1_1 : forall (s2 : result) (st2 : state),
+              ?st =[ ?c1 ]=> st2 / s2 ->
+              ?st' = st2 /\ SContinue = s2,
+    
+    st2: state,
+    H : ?st =[ ?c1 ]=> ?st2 / SBreak |- _ =>
+    destruct (IHHceval1_1 SBreak st2) as [H'] 
+
+  | IHHceval1_1: forall (s2 : result) (st2 : state),
+               ?st =[ ?c1 ]=> st2 / s2 ->
+               ?st' = st2 /\ SContinue = s2,
+                
+    st'0: state,
+    H : ?st =[ ?c1 ]=> ?st'0 / SContinue
+    |- _ =>
+    destruct (IHHceval1_1 SContinue st'0) as [H']
+
+
+  end.
 
 (** **** Exercise: 4 stars, advanced, optional (ceval_deterministic)  *)
 Theorem ceval_deterministic: forall (c:com) st st1 st2 s1 s2,
@@ -1987,7 +2129,20 @@ Theorem ceval_deterministic: forall (c:com) st st1 st2 s1 s2,
      st =[ c ]=> st2 / s2 ->
      st1 = st2 /\ s1 = s2.
 Proof.
-  (* FILL IN HERE *) Admitted.
+  intros c st st1 st2 s1 s2 Hceval1 Hceval2.
+  generalize dependent st2.
+  generalize dependent s2.
+  induction Hceval1; intros s2 st2 Hceval2;
+  inversion Hceval2 as [ | | | | | | | | | ];
+    subst;
+    try (split; reflexivity);
+    try (apply IHHceval1; assumption);
+    try (rewrite H in H0);
+    try discriminate;
+    destruct_IHHceval1_continue;
+    assumption_then_discriminate;
+    assumption_then_solve.
+Qed.
 
 (** [] *)
 End BreakImp.
